#### Q1. Using Library functions, define a function halve::[a] -> ([a],[a]) that splits an even-lengthed list into two halves.For example:

   > halve [1,2,3,4,5,6] <br />
      ([1,2,3],[4,5,6])
    

---

#### Ans:

```haskell
Prelude> :{
Prelude| halve :: [a]-> ([a],[a])
Prelude| halve xs = (take ((length xs) `div` 2) xs , drop ((length xs) `div` 2 )xs)
Prelude| :}
```
**Note:-** *Here you can't use / operator instead of `div` because it may result in floating value which is not acceptable by the in-build take function*


#### Q2. Consider a function safetail::[a]->[a] that behaves as the library function tail, except that safetail maps the empty list to itself, whereas tail produces an error in this. Define safetail using:

#### a) a conditional expression <br />
#### b) guarded equations <br />
#### c) pattern matching <br />

*Hint: make use of the library function null.*

---

#### Ans.

a) **Conditional expression**

```haskell
Prelude> :{
Prelude| safetail :: [a]->[a]
Prelude| safetail as = if (null as) then [] 
Prelude|               else tail as
Prelude| :}
```

b) **Using Gaurded Equation**

```haskell
Prelude> :{
Prelude| safetail :: [a] -> [a]
Prelude| safetail as | (null as) = []
Prelude|             | otherwise = tail as
Prelude| :}

```

c) **Pattern Matching**

```haskell
Prelude> :{
Prelude| safetail :: [a] -> [a]
Prelude| safetail [] =[]
Prelude| safetail as = tail as
Prelude| :}
```

#### Q3. In a similar way to ^, show how the logical disjunction operator || can be defined in four different ways using pattern matching.

---

#### 1st Way.

```haskell
Prelude> :{
Prelude| (||) :: Bool->Bool->Bool
Prelude| True || True = True
Prelude| True || False = True
Prelude| False || True = True
Prelude| False || False = False
Prelude| :}
```

#### 2nd Way

```haskell
Prelude> :{
Prelude| (||) :: Bool->Bool->Bool
Prelude| False || False = False
Prelude| _     || _     = True
Prelude| :}

```

#### 3rd Way

```haskell

Prelude> :{
Prelude| (||) :: Bool -> Bool -> Bool
Prelude| False || b = b
Prelude| True  || _ = True
Prelude| :}

```

#### 4th way

```haskell
Prelude> :{
Prelude| (||) :: Bool -> Bool ->Bool
Prelude| a || b | a==True =True
Prelude|        | b==True = True
Prelude|        | otherwise = False
Prelude| :}

```



#### Q4. Redefine the following version of the conjuction operator using conditional expressions rather than pattern matching:

```haskell
True ^ True = True
_^_         = False

```
---

#### Ans:

```haskell
Prelude> :{
Prelude| (^) :: Bool -> Bool -> Bool
Prelude| a ^ b = if a==True  then 
		    if b==True then True else False
		else False
Prelude| :}
```


#### Q5. Do the same for the following version, and note the difference in the number of conditional expressions required:

 ```haskell
 True ^ b = b
 False ^ _ = False
 ```

---

#### Ans:

```haskell
Prelude> :{
Prelude| (^) :: Bool -> Bool -> Bool
Prelude| a^b = if a==True then b else
Prelude|         False
Prelude| :}

```

#### Q6. Show how the curried function definition mult x y z = x*y*z can be understood in terms of lambda expressions.

---

#### Ans:

```haskell
Prelude> :{
Prelude| mult :: Integer -> Integer -> Integer -> Integer
Prelude| mult = \x -> (\y -> (\z -> x*y*z))
Prelude| :}

```